\documentclass[a4paper,10pt]{amsart}
\usepackage[utf8]{inputenc}
\usepackage{amsmath}
\usepackage{amssymb}
\usepackage{amsthm}
\usepackage{enumerate}
\usepackage{hyperref}
\usepackage{listings}
\usepackage[numbers, comma, sort&compress]{natbib}

\parindent=2em
%opening

\begin{document}
    \author{SDIV, FPA, DGS, GASV}
    \title{Some fucking title}
    \maketitle

    \begin{abstract}
    
    \end{abstract}

    \section{Introduction}
    \section{Model Formulation}
        \paragraph{Hypothesis} We consider that susceptible individuals become 
        infected when they are in contact with asymptomatic individuals and
        individuals with symptoms, we will propose that a proportion of 
        asymptomatic individuals have a way to get relief and not die. A 
        proportion of individuals infected with symptoms may die from the 
        disease or may be relieved. We will introduce two types of control, 
        vaccination of asymptomatic infected and susceptible individuals and 
        treatment of individuals infected with symptoms. 
        \begin{equation}
            \begin{aligned}
                \dot{S}  &= 
                    - \beta \frac{S}{N}(I_s+\alpha I_a) - u S
                \\
                \dot{I_a}  &= 
                    p\beta \frac{S}{N}(I_s + \alpha I_a) - (\rho + u)I_a
                 \\
                \dot{I_s} &=
                    (1 - p) \beta \frac{S}{N} (I_s + \alpha I_a) -
                    (\gamma + \delta + v)I_s
                \\
                \dot{R_a} &= 
                    \rho I_a
                \\
                \dot{R_s} &=
                    \gamma I_s
                \\
                \dot{D} &=
                    \delta I_s
                \\
                \dot{V} &=
                    u(S+I_a)
                \\
                \dot{T} &=
                    v I_s
                \\
                 &
                     S(0) = S_0, 
                     I_a(0) =I_{a_0}, 
                     I_s(0) = I_{s_0}, 
                \\
                 &
                     R_a(0)= R_{a_0}, 
                     R_s(0)= R_{s_0},
                \\
                 &
                     D(0) = D_0,
                     T(0) = T_0,
                \\
                N(t) &= (S+I_a+I_s+R_a+R_s+D+V+T)(t) = cte.           
                \\
                &
                0\leq u(t)\leq u_0, 0\leq v(t)\leq v_0,
            \end{aligned}
        \end{equation}
	\begin{equation}
		J(\vec{x},\vec{u}) = \int^T_0 (I_a(t)+I_s(t)+D(t)+d_1 u(t)+d_2v(t))dt
	\end{equation}
	where 
	\begin{equation*}
	\vec{x}=(S,I_a,I_s,R_a,R_s,D,V,T),\vec{u} =(u,v)
	\end{equation*}
    \section{Adimensional Model}
    \begin{equation}
        \begin{aligned}
        	\dot{\tilde{S}}  &= 
            	- \beta \tilde{S}(\tilde{I}_s
            	+\alpha \tilde{I}_a) - u\tilde{S}
        	\\
        	\dot{E} & = \beta \tilde{S} (\tilde{I}_s + \alpha \tilde{I}_a)   
                 - \kappa E 
            	\\
        	\dot{\tilde{I_a}}  &= 
            	p \kappa \ E 
            	- (\rho+u) \tilde{I}_a
        	\\
        	\dot{\tilde{I_s}} &=
            	(1 - p) \kappa \ E 
            	-( \gamma + \delta + v) \tilde{I}_s
        	\\
        	\dot{\tilde{R_a}} &= 
            	\rho \tilde{I}_a
        	\\
        	\dot{\tilde{R_s}} &=
        	\gamma \tilde{I}_s
        	\\
        	\dot{\tilde{D}} &=
        	\delta \tilde{I}_s
        	\\
        	\dot{\tilde{V}} &=
            u(\tilde{S} + \tilde{I}_a)
        	\\
        	\dot{\tilde{T}} &=
            v \tilde{I}_s
        	\\
            	&
            	\tilde{S}(0) = \tilde{S}_0, 
            	\tilde{I}_a(0) =\tilde{I}_{a_0}, 
            	\tilde{I}_s(0) = \tilde{I}_{s_0}, 
        	\\
        &
            	\tilde{R}_a(0)= \tilde{R}_{a_0}, 
            	\tilde{R}_s(0)= \tilde{R}_{s_0},
        	\\
        &
            \tilde{D}(0) = \tilde{D}_0,
            \tilde{T}(0) = \tilde{T}_0,
        \\
        N(t) &=
        (
            \tilde{S} + \tilde{I}_a + \tilde{I}_s + \tilde{R}_a
            + \tilde{R}_s + \tilde{D} + \tilde{V} + \tilde{T} 
        )(t) = 1.
        \\
        & 0\leq
        \tilde{S},
        \tilde{I}_a,
        \tilde{I}_s,
        \tilde{R}_a,
        \tilde{R}_s,
        \tilde{D},
        \tilde{V}, 
        \tilde{T} \leq 1
        \\
        &
        0\leq u(t)\leq 1, \qquad
        0\leq v(t)\leq 1,
        \end{aligned}
    \end{equation}
    
    \begin{equation}
        J(\vec{\tilde{x}}, \vec{\tilde{u}}) = 
        \int^T_0
            \tilde{I}_a(t) +
            \tilde{I}_s(t) +
            \tilde{D}(t) +
            d_1 u(t) + d_2v(t) 
        dt
    \end{equation}
    
    \section{SEIR version}
       Here we propose a SEIR struture which considers hospitlized 
    compartiment $ H $. To overcome stability issues we also consider 
    vital dynamics.
    \begin{equation}
        \label{eqn:vital_dynamics}
        \begin{aligned}
            \min_{u \in \mathcal{U}} &=
            \int_{0}^T
                \left(
                    a_{I_S} I_S
                    + a_{H} H
                    + a_{D} D
                    + 
                    \frac{a_{L}}{2}  u_L ^ 2
                    + 
                    \frac{a_{V}}{2} u_V ^ 2 
                    + 
                    \frac{a_{H}}{2} u_H ^ 2 
                    + 
                    \frac{a_{M}}{2} u_M ^ 2 
                \right)
                dt
            \\
            \text{s. t.}
            \\
            L' & = 
                -\epsilon \lambda L - u_L(t) L - \mu L
            \\
            S' & =
                \mu N^\star + u_L(t) L + (1 - \widehat{q}) \gamma_V V 
                - \lambda S - u_V(t) S - \mu S
            \\
            E' & =
                \lambda (\epsilon L + S) - \kappa E - \mu E
            \\
            I_S' & =
                p \kappa E - (\gamma_S + \mu_{I_S} + \delta_H) I_S 
                - u_M(t) I_S + (1 - q) \gamma_M M(t)
                - \mu I_S
            \\
            I_A' &=
                (1 - p) \kappa E - \gamma_A I_A - \mu I_A
            \\
            M' &=
                u_M(t) I_S - \gamma_M M - \mu M
            \\
            H' &=
                \delta_H I_S - (\gamma_H + \mu_H) H - u_H(t) H - \mu H
            \\
            R' & =
                \gamma_S I_S + \gamma_A I_A + \gamma_H H + q \gamma_M M
                + u_H(t) H + \widehat{q} \gamma_V V - \mu R
            \\
            D' &=
                \mu_{I_S} I_S + \mu_H H
            \\
            V' &=
                u_V(t) S  - \gamma_V  V  - \mu V
            \\
            \lambda &:=
                \frac{\beta_A I_A + \beta_S I_S}{N^{\star}}
            \\
            N^{\star}(t) &=
                L + S +E + I_S + I_A +
                M + H + R + V
        \end{aligned}
    \end{equation}
    \paragraph{Minima Squares}
        \paragraph{Likelihood}
        \paragraph{Bayesian}
    \section{Optimal control problem}
    \section{Numerical Results}
\end{document}
